WIP

Phi_Algebras/Phi_Spec_Pre.thy
@@ -9,5 +9,15 @@ lemma Subjection_expn:
   "p \<in> (T \<s>\<u>\<b>\<j> P) \<longleftrightarrow> p \<in> T \<and> P"
   unfolding Subjection_def by simp
 
+lemma Subjection_Id_on:
+  \<open>Id_on (S \<s>\<u>\<b>\<j> P) = (Id_on S \<s>\<u>\<b>\<j> P)\<close>
+  by (auto simp add: Subjection_expn)
+
+definition ExSet :: " ('c \<Rightarrow> 'a set) \<Rightarrow> 'a set" (binder "\<exists>*" 14)
+  where "ExSet S = {p. (\<exists>c. p \<in> S c)}"
+notation ExSet (binder "\<exists>\<^sup>s" 14)
+
+lemma ExSet_expn: "p \<in> ExSet S \<longleftrightarrow> (\<exists>c. p \<in> S c)" unfolding ExSet_def by simp
+
 
 end
